Move a bunch of stuff to Tactics/Prelude
General code hygiene
Switched Typing to use the conv from Reduction

Reduction.v
@@ -27,10 +27,12 @@ Require Import Scoping.
 Notation env a := (Expr.name -> option a).
 Reserved Notation "a ::> b" (at level 50).
 Variable const_vals : env exp.
+Hypothesis const_vals_closed : forall nm e, const_vals nm = Some e -> closed e.
+Hint Resolve const_vals_closed.
 
 Inductive par_step : relation exp :=
 | P_ref    : forall e, e ::> e
-(* | P_free   : forall nm e, const_vals nm = Some e -> Free nm ::> e                     *)
+| P_free   : forall nm e, const_vals nm = Some e -> Free nm ::> e
 
 | P_pi     : forall A A' B B', A ::> A' -> B ::> B' -> A :>> B ::> A' :>> B'
 (* | P_lam    : forall A A' b b', A ::> A' -> b ::> b' -> A :#> b ::> A' :#> b' *)
@@ -76,7 +78,7 @@ Hypothesis consts_closed : forall nm e, const_vals nm = Some e -> closed e.
 
 Fixpoint rho (e : exp) : exp :=  
   match e with
-    (* | Free nm => match const_vals nm with None => Free nm | Some e => e end *)
+    | Free nm => match const_vals nm with None => Free nm | Some e => e end
     | (A :>> B) => (rho A) :>> (rho B)
     | (Lam b) => Lam (rho b)
     | (f :$: a) => match rho f with
@@ -126,9 +128,11 @@ Fixpoint rho (e : exp) : exp :=
 
 Hint Constructors par_step.
 
-Fixpoint rho_eval_to e : e ::> rho e.
-Proof. induction e; simpl; try destruct match; eauto. Qed.
-
+Lemma rho_eval_to e : e ::> rho e.
+Proof. induction e; simpl; try solve[try destruct match;eauto].
+  remember (const_vals n) as cn; symmetry in Heqcn.
+  destruct cn; auto.
+Qed.
 Hint Resolve rho_eval_to.
 
 Tactic Notation "invert" "value" "steps" :=
@@ -148,7 +152,7 @@ Tactic Notation "invert" "value" "steps" :=
   end.
 
 Notation spstep sigma tau := (forall v, sigma v ::> tau v).
-Infix ".>>" := spstep (at level 50).
+Infix ".>" := spstep (at level 50).
 
 Hint Rewrite up_lift1 up_liftn.
 Lemma wk_up : forall c, wk 1 >> up c = c >> wk 1. intros; autosubst. Qed.
@@ -163,8 +167,8 @@ Hint Rewrite closed_sub_id using (auto; fail).
 
 Definition efunc_closed : forall D e, closed e -> closed (D_efunc D e).
 Proof. induction D; intros; simpl; rewrite asms; auto; simpl.
-       try_hyps; clear_funs; replace (D_efunc D2 e).[wk 1] with (D_efunc D2 e) by (autorewrite with core; auto).
-       eapply closed_lift; try eassumption; auto.
+  try_hyps; clear_funs; replace (D_efunc D2 e).[wk 1] with (D_efunc D2 e) by (autorewrite with core; auto).
+  eapply closed_lift; try eassumption; auto.
 Qed.
 
 Lemma sub_sig_scop : forall e sigma i j, sub_vars i j sigma -> closed_at j e -> sub_vars i.+1 j (e .: sigma).
@@ -176,48 +180,46 @@ Hint Resolve sub_ids_scop.
 
 Definition rall_scoped : forall D r e n, closed_at n.+1 r -> closed_at n e -> closed_at n (rall D r e).
 Proof. induction D; intros; simpl; rewrite asms; auto; simpl; auto;
-       apply sub_vars_corr with (i := n.+1); auto; 
-       apply sub_sig_scop || apply sub_up_vars; auto.
+  apply sub_vars_scoped with (i := n.+1); auto; 
+  apply sub_sig_scop || apply sub_up_vars; auto.
 Qed.
-       
-Hint Resolve efunc_closed rall_scoped.
+
 Hint Constructors par_step.
 
 Lemma rall_sub D : forall r e sigma, (rall D r e).[sigma] = rall D r.[up sigma] e.[sigma].
 Proof. induction D; intros; auto; simpl; rewrite asms; autosubst. Qed.
-  
 Hint Rewrite rall_sub.   
 
+Hint Extern 1 (Free ?nm ::> ?e.[_]) => rewrite closed_sub_id; [constructor|eapply const_vals_closed]; eassumption.
+Hint Extern 1 (const_vals ?nm = Some ?e.[_]) => rewrite closed_sub_id; try eapply const_vals_closed; eassumption.
+Hint Resolve closed_sub_id.
 Lemma sub_cong1 : forall e1 e2, e1 ::> e2 -> forall sigma, e1.[sigma] ::> e2.[sigma].
 Proof. induction 1; intros; simpl in *;
-  rewrite ?rall_sub; simpl; autorewrite with core; try constructor; solve[eauto].
+  rewrite ?rall_sub; simpl; autorewrite with core; try solve[try constructor; eauto].
 Qed.
-
 Local Hint Resolve sub_cong1.
-Notation sstep sigma tau :=(forall v, sigma v ::> tau v).
-Infix ".>>" := spstep (at level 50).
 
-Lemma subst_up : forall c1 c2, c1 .>> c2 -> up c1 .>> up c2.
+Lemma subst_up : forall c1 c2, c1 .> c2 -> up c1 .> up c2.
 Proof. intros. destruct v; asimpl; auto. Qed.
 
 Hint Resolve subst_up.
 
-Lemma sub_cong2 : forall e c1 c2, c1 .>> c2 -> e.[c1] ::> e.[c2].
+Lemma sub_cong2 : forall e c1 c2, c1 .> c2 -> e.[c1] ::> e.[c2].
 Proof. induction e; intros; simpl in *; try econstructor; eauto. Qed.
 
 Local Hint Resolve sub_cong2.
 
-Lemma sub_cong : forall e1 e2, e1 ::> e2 -> forall c1 c2, c1 .>> c2 -> e1.[c1] ::> e2.[c2].
+Lemma sub_cong : forall e1 e2, e1 ::> e2 -> forall c1 c2, c1 .> c2 -> e1.[c1] ::> e2.[c2].
 Proof. induction 1; intros; simpl in *; try solve [auto];
   repeat (simpl; autorewrite with core); try solve [econstructor; eauto].
 Qed.
 
 Hint Resolve sub_cong.
 
-Lemma sub_cons : forall e e' sigma tau, e ::> e' -> sigma .>> tau -> (e .: sigma) .>> (e' .: tau). destruct v; simpl; auto. Qed.
+Lemma sub_cons : forall e e' sigma tau, e ::> e' -> sigma .> tau -> (e .: sigma) .> (e' .: tau). destruct v; simpl; auto. Qed.
 
-Lemma ids_ev : ids .>> ids. auto. Qed.
-Lemma up_ev : forall sigma tau, sigma .>> tau -> up sigma .>> up tau. destruct v; simpl; auto. Qed.
+Lemma ids_ev : ids .> ids. auto. Qed.
+Lemma up_ev : forall sigma tau, sigma .> tau -> up sigma .> up tau. destruct v; simpl; auto. Qed.
 
 Hint Resolve ids_ev up_ev sub_cons.
 
@@ -226,7 +228,9 @@ Lemma rall_ev D : forall r r', r ::> r' -> forall e e', e ::>  e' -> rall D r e 
 Hint Resolve rall_ev.
 
 Lemma rho_eval_from_to e e' : e ::> e' -> e' ::> rho e.
-Proof. induction 1; simpl; try (invert value steps || destruct match); eauto 10. Qed.
+Proof. induction 1; simpl; try (invert value steps || destruct match); eauto 10; try solve by inversion.
+  inverts H; auto.
+Qed.
 
 Hint Resolve rho_eval_from_to.
 
@@ -238,67 +242,75 @@ Infix ":::>" := red (at level 50).
 Local Hint Resolve t_step rst_step rst_refl.
 Local Hint Resolve t_trans rst_trans rst_sym : slow.
 
-Lemma red_Pi_l : forall A B A', A :::> A' -> Pi A B :::> Pi A' B. induction 1; eauto with slow. Qed.
-Lemma red_Pi_r : forall A B B', B :::> B' -> Pi A B :::> Pi A B'. induction 1; eauto with slow. Qed.
+Lemma red_Pi_l : forall A B A', A :::> A' -> Pi A B :::> Pi A' B. induction 1; eauto. Qed.
+Lemma red_Pi_r : forall A B B', B :::> B' -> Pi A B :::> Pi A B'. induction 1; eauto. Qed.
 Local Hint Resolve red_Pi_l red_Pi_r.
 
-Lemma red_Pi_Pi A B A' B' : (A :::> A') -> (B :::> B') -> Pi A B :::> Pi A' B'. eauto with slow. Qed.
+Lemma red_Pi_Pi A B A' B' : (A :::> A') -> (B :::> B') -> Pi A B :::> Pi A' B'. eauto. Qed.
 Hint Resolve red_Pi_Pi.
 
-Lemma red_Sigma_l : forall A B A', A :::> A' -> Sigma A B :::> Sigma A' B. induction 1; eauto with slow. Qed.
-Lemma red_Sigma_r : forall A B B', B :::> B' -> Sigma A B :::> Sigma A B'. induction 1; eauto with slow. Qed.
+Lemma red_Sigma_l : forall A B A', A :::> A' -> Sigma A B :::> Sigma A' B. induction 1; eauto. Qed.
+Lemma red_Sigma_r : forall A B B', B :::> B' -> Sigma A B :::> Sigma A B'. induction 1; eauto. Qed.
 Local Hint Resolve red_Sigma_l red_Sigma_r.
  
-Lemma red_Sigma_Sigma A B A' B' : (A :::> A') -> (B :::> B') -> Sigma A B :::> Sigma A' B'. eauto with slow. Qed.
+Lemma red_Sigma_Sigma A B A' B' : (A :::> A') -> (B :::> B') -> Sigma A B :::> Sigma A' B'. eauto. Qed.
 Hint Resolve red_Sigma_Sigma.
 
-Lemma red_Sum_l : forall A B A', A :::> A' -> Sum A B :::> Sum A' B. induction 1; eauto with slow. Qed.
-Lemma red_Sum_r : forall A B B', B :::> B' -> Sum A B :::> Sum A B'. induction 1; eauto with slow. Qed.
+Lemma red_Sum_l : forall A B A', A :::> A' -> Sum A B :::> Sum A' B. induction 1; eauto. Qed.
+Lemma red_Sum_r : forall A B B', B :::> B' -> Sum A B :::> Sum A B'. induction 1; eauto. Qed.
 Local Hint Resolve red_Sum_l red_Sum_r.
 
-Lemma red_Sum_Sum A B A' B' : (A :::> A') -> (B :::> B') -> Sum A B :::> Sum A' B'. eauto with slow. Qed.
+Lemma red_Sum_Sum A B A' B' : (A :::> A') -> (B :::> B') -> Sum A B :::> Sum A' B'. eauto. Qed.
 Hint Resolve red_Sum_Sum.
 
-Lemma red_Lam_Lam : forall e e', e :::> e' -> Lam e :::> Lam e'. induction 1; eauto with slow. Qed.
+Lemma red_Lam_Lam : forall e e', e :::> e' -> Lam e :::> Lam e'. induction 1; eauto. Qed.
 Hint Resolve red_Lam_Lam.
 
-Lemma red_S_p1_S_p1 : forall e e', e :::> e' -> S_p1 e :::> S_p1 e'. induction 1; eauto with slow. Qed.
-Lemma red_S_p2_S_p2 : forall e e', e :::> e' -> S_p2 e :::> S_p2 e'. induction 1; eauto with slow. Qed.
+Lemma red_S_p1_S_p1 : forall e e', e :::> e' -> S_p1 e :::> S_p1 e'. induction 1; eauto. Qed.
+Lemma red_S_p2_S_p2 : forall e e', e :::> e' -> S_p2 e :::> S_p2 e'. induction 1; eauto. Qed.
 Hint Resolve red_S_p1_S_p1 red_S_p2_S_p2.
 
-Lemma red_Sum_inl_Sum_inl : forall e e', e :::> e' -> Sum_inl e :::> Sum_inl e'. induction 1; eauto with slow. Qed.
-Lemma red_Sum_inr_Sum_inr : forall e e', e :::> e' -> Sum_inr e :::> Sum_inr e'. induction 1; eauto with slow. Qed.
+Lemma red_Sum_inl_Sum_inl : forall e e', e :::> e' -> Sum_inl e :::> Sum_inl e'. induction 1; eauto. Qed.
+Lemma red_Sum_inr_Sum_inr : forall e e', e :::> e' -> Sum_inr e :::> Sum_inr e'. induction 1; eauto. Qed.
 Hint Resolve red_Sum_inl_Sum_inl red_Sum_inr_Sum_inr.
 
-Lemma red_App_l : forall A B A', A :::> A' -> App A B :::> App A' B. induction 1; eauto with slow. Qed.
-Lemma red_App_r : forall A B B', B :::> B' -> App A B :::> App A B'. induction 1; eauto with slow. Qed.
+Lemma red_App_l : forall A B A', A :::> A' -> App A B :::> App A' B. induction 1; eauto. Qed.
+Lemma red_App_r : forall A B B', B :::> B' -> App A B :::> App A B'. induction 1; eauto. Qed.
 Local Hint Resolve red_App_l red_App_r.
 
-Lemma red_App_App A B A' B' : (A :::> A') -> (B :::> B') -> App A B :::> App A' B'. eauto with slow. Qed.
+Lemma red_App_App A B A' B' : (A :::> A') -> (B :::> B') -> App A B :::> App A' B'. eauto. Qed.
 Hint Resolve red_App_App.
 
-Lemma red_S_mk_l : forall A B A', A :::> A' -> S_mk A B :::> S_mk A' B. induction 1; eauto with slow. Qed.
-Lemma red_S_mk_r : forall A B B', B :::> B' -> S_mk A B :::> S_mk A B'. induction 1; eauto with slow. Qed.
+Lemma red_S_mk_l : forall A B A', A :::> A' -> S_mk A B :::> S_mk A' B. induction 1; eauto. Qed.
+Lemma red_S_mk_r : forall A B B', B :::> B' -> S_mk A B :::> S_mk A B'. induction 1; eauto. Qed.
 Local Hint Resolve red_S_mk_l red_S_mk_r.
 
-Lemma red_S_mk_S_mk a b a' b' : a :::> a' -> b :::> b' -> S_mk a b :::> S_mk a' b'. eauto with slow. Qed.
+Lemma red_S_mk_S_mk a b a' b' : a :::> a' -> b :::> b' -> S_mk a b :::> S_mk a' b'. eauto. Qed.
 Hint Resolve red_S_mk_S_mk.
 
-Lemma red_Split_1 a b c a' : (a :::> a') -> Split a b c :::> Split a' b c. induction 1; eauto with slow. Qed.
-Lemma red_Split_2 a b c b' : (b :::> b') -> Split a b c :::> Split a b' c. induction 1; eauto with slow. Qed.
-Lemma red_Split_3 a b c c' : (c :::> c') -> Split a b c :::> Split a b c'. induction 1; eauto with slow. Qed.
+Lemma red_Split_1 a b c a' : (a :::> a') -> Split a b c :::> Split a' b c. induction 1; eauto. Qed.
+Lemma red_Split_2 a b c b' : (b :::> b') -> Split a b c :::> Split a b' c. induction 1; eauto. Qed.
+Lemma red_Split_3 a b c c' : (c :::> c') -> Split a b c :::> Split a b c'. induction 1; eauto. Qed.
 Local Hint Resolve red_Split_1 red_Split_2 red_Split_3.
 
 Lemma red_Split_Split a b c a' b' c' : (a :::> a') -> (b :::> b') -> (c :::> c') -> Split a b c :::> Split a' b' c'.
-Proof. intros. apply t_trans with (y := Split a' b c); eauto with slow. Qed.
+Proof. intros. transitivity (Split a' b c); eauto. Qed.
 Hint Resolve red_Split_Split.
 
-Lemma red_mu_l D : forall A B A', A :::> A' -> mu D A B :::> mu D A' B. induction 1; eauto with slow. Qed.
-Lemma red_mu_r D : forall A B B', B :::> B' -> mu D A B :::> mu D A B'. induction 1; eauto with slow. Qed.
+Lemma red_mu_l D : forall A B A', A :::> A' -> mu D A B :::> mu D A' B. induction 1; eauto. Qed.
+Lemma red_mu_r D : forall A B B', B :::> B' -> mu D A B :::> mu D A B'. induction 1; eauto. Qed.
 Local Hint Resolve red_mu_l red_mu_r.
 
-Lemma red_mu_mu D A B A' B' : (A :::> A') -> (B :::> B') -> mu D A B :::> mu D A' B'. eauto with slow. Qed.
+Lemma red_mu_mu D A B A' B' : (A :::> A') -> (B :::> B') -> mu D A B :::> mu D A' B'. eauto. Qed.
 Hint Resolve red_mu_mu.
+
+Lemma red_Free nm e : Free nm :::> e <-> (e = Free nm) \/ (exists v, const_vals nm = Some v /\ v :::> e).
+Proof. remember (Free nm).
+  split; induction 1; subst; auto.
+  - + inverts H; eauto.
+    + intuition; subst; destr_logic; eauto.
+  - destr_logic; eauto.
+Qed.
 
 Lemma red_Bind v e : Bind v :::> e <-> e = Bind v. 
 Proof. remember (Bind v).
@@ -335,7 +347,7 @@ Proof. split.
     induction Hab; intros; subst; auto.
     { inversion H; subst; eauto 10. }
     { specialize (IHHab1 A B); intuition; destr_logic; subst.
-      specialize (IHHab2 x x0); intuition; destr_logic; subst. eauto 10 with slow. } }
+      specialize (IHHab2 x x0); intuition; destr_logic; subst. eauto 10. } }
   { intros; destr_logic; subst; auto. }
 Qed.
 
@@ -346,7 +358,7 @@ Proof. split.
     induction Hab; intros; subst; auto.
     { inversion H; subst; eauto 10. }
     { specialize (IHHab1 A B); intuition; destr_logic; subst.
-      specialize (IHHab2 x x0); intuition; destr_logic; subst. eauto 10 with slow. } }
+      specialize (IHHab2 x x0); intuition; destr_logic; subst. eauto 10. } }
   { intros; destr_logic; subst; auto. }
 Qed.
 
@@ -357,7 +369,7 @@ Proof. split.
     induction Hab; intros; subst; auto.
     { inversion H; subst; eauto 10. }
     { specialize (IHHab1 A B); intuition; destr_logic; subst.
-      specialize (IHHab2 x x0); intuition; destr_logic; subst. eauto 10 with slow. } }
+      specialize (IHHab2 x x0); intuition; destr_logic; subst. eauto 10. } }
   { intros; destr_logic; subst; auto. }
 Qed.
 
@@ -368,7 +380,7 @@ Proof. split.
     induction Hab; intros; subst; auto.
     { inversion H; subst; eauto 10. }
     { specialize (IHHab1 A B); intuition; destr_logic; subst.
-      specialize (IHHab2 x x0); intuition; destr_logic; subst. eauto 10 with slow. } }
+      specialize (IHHab2 x x0); intuition; destr_logic; subst. eauto 10. } }
   { intros; destr_logic; subst; auto. }
 Qed.
 
@@ -412,18 +424,20 @@ Lemma sred_cong1 : forall e e' sigma, e :::> e' -> e.[sigma] :::> e'.[sigma]. in
 Local Hint Resolve sred_cong1.
 
 Notation sred sigma tau := (forall i : var, sigma i :::> tau i).
-Infix ".>>>" := sred (at level 50).
+Infix "..>" := sred (at level 50).
 
-Lemma sred_ref : forall sigma, sigma .>>> sigma. intros; eauto. Qed.
-Lemma sub_sred : forall sigma tau, sigma .>>> tau -> forall e e', e :::> e' -> (e .: sigma) .>>> (e' .: tau). intros; destruct i; simpl; auto. Qed.
+Lemma sred_ref : forall sigma, sigma ..> sigma. intros; eauto. Qed.
+Lemma sub_sred : forall sigma tau, sigma ..> tau -> forall e e', e :::> e' -> (e .: sigma) ..> (e' .: tau). intros; destruct i; simpl; auto. Qed.
 
-Lemma up_sred : forall sigma tau, sigma .>>> tau -> up sigma .>>> up tau. intros; destruct i; asimpl; auto. Qed.
+Lemma sred_trans : forall delta sigma tau, delta ..> sigma -> sigma ..> tau -> delta ..> tau. eauto. Qed.
+
+Lemma up_sred : forall sigma tau, sigma ..> tau -> up sigma ..> up tau. intros; destruct i; asimpl; auto. Qed.
 Hint Resolve up_sred sub_sred sred_ref.
 
-Lemma sred_cong2 : forall e sigma tau, sigma .>>> tau -> e.[sigma] :::> e.[tau]. induction e; intros; simpl; auto. Qed.
+Lemma sred_cong2 : forall e sigma tau, sigma ..> tau -> e.[sigma] :::> e.[tau]. induction e; intros; simpl; auto. Qed.
 Local Hint Resolve sred_cong2.
 
-Lemma sred_cong : forall e e', e :::> e' -> forall sigma tau, sigma .>>> tau -> e.[sigma] :::> e'.[tau]. intros. apply t_trans with (y := e.[tau]); auto. Qed.
+Lemma sred_cong : forall e e', e :::> e' -> forall sigma tau, sigma ..> tau -> e.[sigma] :::> e'.[tau]. intros. apply t_trans with (y := e.[tau]); auto. Qed.
 Hint Resolve sred_cong.
 
 Lemma red_App f a e : (f :$: a) :::> e <-> (exists f' a', e = (f' :$: a') /\ (f :::> f') /\ (a :::> a')) \/
@@ -501,7 +515,7 @@ Proof. split.
     eapply t_trans with (y := _ :$: _ :$: _); try eassumption; eauto. }
 Qed.
 
-Hint Rewrite red_App red_S_p1 red_S_p2 red_Split red_mu : beta.
+Hint Rewrite red_Free red_App red_S_p1 red_S_p2 red_Split red_mu : beta.
 
 Lemma red_conv : forall e e', e :::> e' -> e <:::> e'. induction 1; eauto with slow. Qed.
 Hint Resolve red_conv.
@@ -527,7 +541,7 @@ Lemma conv_double_red : forall e1 e2, e1 <:::> e2 <-> (exists e3, e1 :::> e3 /\ 
 Proof.
   split; move=>H; [|destr_logic; eauto with slow].
   induction H; try solve[eauto].
-  - destr_logic; solve[eauto with slow].
+  - destr_logic; solve[eauto].
   - destr_logic. extend red_confl.
     try_hyps; clear_funs; destr_logic; solve[eauto].
 Qed.
@@ -535,13 +549,149 @@ Qed.
 (* Hint Resolve conv_double_red. *) (* not hinting because red_confl caused problems *)
 Hint Rewrite conv_double_red : unconv.
 
-(* Not working for now - need to add P_free rule *)
-(* Lemma red_Free nm e : Free nm :::> e <-> (e = Free nm) \/ (exists e', const_vals nm = Some e' /\ e' :::> e). *)
-(* Proof. split. *)
-(*   { remember (Free nm) as f.  *)
-(*     induction 1; subst. *)
-(*     - inversion H; subst; eauto. *)
-(*     - specialize (IHclos_trans1 erefl); destr_logic; subst; eauto. } *)
-(*   { destruct 1; subst; destr_logic; eauto. *)
-(*     apply t_trans with (y := x); auto. } *)
-(* Qed. *)
+Notation sconv sigma tau := (forall i, sigma i <:::> tau i).
+Infix "<..>" := sconv (at level 20).
+
+Lemma conv_Bind_iff i j : Bind i <:::> Bind j <-> i = j. 
+Proof. autorewrite with unconv; split; intros; destr_logic; autorewrite with core in *; destr_logic; subst; congruence || eauto. Qed.
+
+Lemma conv_Sort_iff i j : Sort i <:::> Sort j <-> i = j. 
+Proof. autorewrite with unconv; split; intros; destr_logic; autorewrite with core in *; destr_logic; subst; congruence || eauto. Qed.
+
+Lemma conv_Mu_iff D1 D2 : Mu D1 <:::> Mu D2 <-> D1 = D2.
+Proof. autorewrite with unconv; split; intros; destr_logic; autorewrite with core in *; destr_logic; subst; congruence || eauto. Qed.
+
+Hint Rewrite conv_Bind_iff conv_Sort_iff conv_Mu_iff.
+
+Lemma conv_Lam_iff b1 b2 : Lam b1 <:::> Lam b2 <-> b1 <:::> b2.
+Proof. autorewrite with unconv; split; intros; destr_logic; autorewrite with core in *; destr_logic; eauto.
+  subst; inversion H0; subst; eauto.
+Qed.
+
+Lemma conv_Sum_inl_iff b1 b2 : Sum_inl b1 <:::> Sum_inl b2 <-> b1 <:::> b2.
+Proof. autorewrite with unconv; split; intros; destr_logic; autorewrite with core in *; destr_logic; eauto.
+  subst; inversion H0; subst; eauto.
+Qed.
+
+Lemma conv_Sum_inr_iff b1 b2 : Sum_inr b1 <:::> Sum_inr b2 <-> b1 <:::> b2.
+Proof. autorewrite with unconv; split; intros; destr_logic; autorewrite with core in *; destr_logic; eauto.
+  subst; inversion H0; subst; eauto.
+Qed.
+
+Hint Rewrite conv_Lam_iff conv_Sum_inl_iff conv_Sum_inr_iff.
+
+Lemma conv_Pi_iff A B A' B' : (Pi A B <:::> Pi A' B') <-> (A <:::> A' /\ B <:::> B').
+Proof. autorewrite with unconv; split; intros; destr_logic; autorewrite with core in *; destr_logic; eauto.
+  subst. inversion H0; subst. split; eauto.
+Qed.
+
+Lemma conv_Sigma_iff A B A' B' : (Sigma A B <:::> Sigma A' B') <-> (A <:::> A' /\ B <:::> B').
+Proof. autorewrite with unconv; split; intros; destr_logic; autorewrite with core in *; destr_logic; eauto.
+  subst. inversion H0; subst. split; eauto.
+Qed.
+
+Lemma conv_Sum_iff A B A' B' : (Sum A B <:::> Sum A' B') <-> (A <:::> A' /\ B <:::> B').
+Proof. autorewrite with unconv; split; intros; destr_logic; autorewrite with core in *; destr_logic; eauto.
+  subst. inversion H0; subst. split; eauto.
+Qed.
+
+Lemma conv_S_mk_iff A B A' B' : (S_mk A B <:::> S_mk A' B') <-> (A <:::> A' /\ B <:::> B').
+Proof. autorewrite with unconv; split; intros; destr_logic; autorewrite with core in *; destr_logic; eauto.
+  subst. inversion H0; subst. split; eauto.
+Qed.
+
+Hint Rewrite conv_Pi_iff conv_Sigma_iff conv_Sum_iff conv_S_mk_iff.
+
+Lemma conv_Pi_Pi A B A' B' : A <:::> A' -> B <:::> B' -> Pi A B <:::> Pi A' B'.
+Proof. autorewrite with core; auto. Qed.
+
+Lemma conv_Sigma_Sigma A B A' B' : A <:::> A' -> B <:::> B' -> Sigma A B <:::> Sigma A' B'.
+Proof. autorewrite with core; auto. Qed.
+
+Lemma conv_Sum_Sum A B A' B' : A <:::> A' -> B <:::> B' -> Sum A B <:::> Sum A' B'.
+Proof. autorewrite with core; auto. Qed.
+
+Lemma conv_S_mk_S_mk A B A' B' : A <:::> A' -> B <:::> B' -> S_mk A B <:::> S_mk A' B'.
+Proof. autorewrite with core; auto. Qed.
+
+Lemma conv_Lam_Lam : forall b1 b2, b1 <:::> b2 -> Lam b1 <:::> Lam b2. intros; autorewrite with core; auto. Qed.
+
+Hint Resolve conv_Pi_Pi conv_Sigma_Sigma conv_Sum_Sum conv_S_mk_S_mk conv_Lam_Lam.
+
+Lemma conv_S_p1_S_p1 : forall e e', e <:::> e' -> S_p1 e <:::> S_p1 e'.
+Proof. intros; autorewrite with unconv in *; destr_logic; eauto. Qed.
+
+Lemma conv_S_p2_S_p2 : forall e e', e <:::> e' -> S_p2 e <:::> S_p2 e'.
+Proof. intros; autorewrite with unconv in *; destr_logic; eauto. Qed.
+
+Hint Resolve conv_S_p1_S_p1 red_S_p2_S_p2.
+
+Lemma conv_Sum_inl_Sum_inl : forall e e', e <:::> e' -> Sum_inl e <:::> Sum_inl e'. intros; autorewrite with core; auto. Qed.
+Lemma conv_Sum_inr_Sum_inr : forall e e', e <:::> e' -> Sum_inr e <:::> Sum_inr e'. intros; autorewrite with core; auto. Qed.
+Hint Resolve conv_Sum_inl_Sum_inl conv_Sum_inr_Sum_inr.
+
+
+Lemma conv_App_App f a f' a' : (f <:::> f') -> (a <:::> a') -> ((f :$: a) <:::> (f' :$: a')).
+Proof. autorewrite with unconv; intros; destr_logic; autorewrite with core in *; destr_logic; eauto. Qed.
+Hint Resolve conv_App_App.
+
+Lemma conv_Split_Split a b c a' b' c' : (a <:::> a') -> (b <:::> b') -> (c <:::> c') -> Split a b c <:::> Split a' b' c'.
+Proof. autorewrite with unconv; intros; destr_logic; autorewrite with core in *; destr_logic; eauto. Qed.
+Hint Resolve conv_Split_Split.
+
+Lemma conv_mu_mu D A B A' B' : (A <:::> A') -> (B <:::> B') -> mu D A B <:::> mu D A' B'.
+Proof. autorewrite with unconv; intros; destr_logic; autorewrite with core in *; destr_logic; eauto. Qed.
+Hint Resolve conv_mu_mu.
+
+Lemma sconv_cong1 sigma e1 e2 : e1 <:::> e2 -> e1.[sigma] <:::> e2.[sigma].
+Proof. autorewrite with unconv; intros; destr_logic; eauto. Qed.
+Hint Resolve sconv_cong1.
+
+Lemma sub_up sigma tau : sigma <..> tau -> up sigma <..> up tau.
+Proof. intros; destruct i; asimpl; auto. Qed.
+Hint Resolve sub_up.
+
+Lemma sconv_cong2 e : forall sigma tau, sigma <..> tau -> e.[sigma] <:::> e.[tau].
+Proof. induction e; simpl; auto 10.
+  - intros; apply conv_S_p2_S_p2; auto. (* for some reason this case doesn't work on its own *)
+Qed.
+Hint Resolve sconv_cong2.
+
+Lemma sconv_cong e1 e2 sigma tau : e1 <:::> e2 -> sigma <..> tau -> e1.[sigma] <:::> e2.[tau]. intros; transitivity (e1.[tau]); auto. Qed.
+
+Definition subtyp A B := (A <:::> B \/ exists i j, A <:::> Sort i /\ B <:::> Sort j /\ i < j).
+Infix "::<<" := subtyp (at level 20).
+
+Lemma conv_sort_red e i : e <:::> Sort i <-> e :::> Sort i.
+Proof. split; [|auto]. autorewrite with unconv; intros; destr_logic; autorewrite with core in *; subst; auto. Qed.
+(* Hint Resolve conv_sort_red. *)
+Hint Rewrite conv_sort_red : unconv.
+
+Hint Resolve red_conv.
+Lemma conv_ext_l e1 e2 e3 : e1 <:::> e2 -> e2 :::> e3 -> e1 <:::> e3. eauto using clos_refl_sym_trans. Qed.
+Lemma conv_ext_r e1 e2 e3 : e1 :::> e2 -> e2 <:::> e3 -> e1 <:::> e3. eauto using clos_refl_sym_trans. Qed.
+Hint Resolve conv_ext_l conv_ext_r : slow.
+
+Instance subtyp_refl : Reflexive subtyp. unfold subtyp; auto. Qed.
+
+Hint Resolve sconv_cong1 sconv_cong2 sconv_cong.
+
+Tactic Notation "eauto" "rst" := eauto using clos_refl_sym_trans.
+Tactic Notation "eauto" "rst" integer(n) := eauto n using clos_refl_sym_trans.
+Instance subtyp_trans : Transitive subtyp. 
+Proof. repeat destruct 1; destr_logic; autorewrite with core in *.
+  - left; eauto rst.
+  - right; eauto rst 7.
+  - assert (z <:::> Sort x1) by eauto using rst_trans,rst_sym.
+    right; eauto 7.
+  - assert (Sort x3 <:::> Sort x0) by eauto rst.
+    autorewrite with core in *; subst.
+    right; exists x2; exists x1; repeat split; [eauto rst|eauto rst|transitivity x0]; auto.
+Qed.
+
+Lemma subtyp_cong1 A B sigma : subtyp A B -> subtyp A.[sigma] B.[sigma]. 
+Proof. destruct 1; [left|right]; destr_logic; auto.
+  repeat eexists;
+  match goal with [|-context[Sort ?i]] => change (Sort i) with (Sort i).[sigma] | _ => eassumption end;
+  auto.
+Qed.
