Typing.v
@@ -1,39 +1,22 @@
 Require Import Prelude.
-Require Import Expr.
-Require Import Scoping.
+Require Import Expr. 
+Require Import Scoping. 
+Require Import Reduction.
+
+Notation typ := exp.
+Notation con := (seq exp).
+Inductive subtyp : typ -> typ -> Prop :=
+| sub_conv : forall T1 T2, T1 <:::> T2 -> subtyp T1 T2
+| sub_cumu : forall T1 l1 l2 T2, T1 <:::> (Sort l1) -> T2 <:::> (Sort l2) -> l1 < l2 -> subtyp T1 T2.
+
+Hint Constructors subtyp.
+Infix "::<" := subtyp (at level 20).
+
+Hint Resolve sub_conv.
 Hint Resolve leP ltP eqP.
 
-Fixpoint map_with_ix {A B} (f : nat -> A -> B) (xs : seq A) : seq B :=
-  match xs with
-      [] => []
-    | x :: xs' => f 0 x :: map_with_ix (fun n a => f n.+1 a) xs'
-  end.
-
-Lemma map_with_ix_funext {A B} xs : forall (f g : nat -> A -> B), (forall n a, f n a = g n a) -> map_with_ix f xs = map_with_ix g xs.
-  induction xs; intros; simpl; f_equal; auto. Qed.
-Hint Rewrite @map_with_ix_funext using solve [eauto].
-Hint Rewrite @iterate_S @iterate_0.
-
-Ltac bdestruct X :=
-  let H := fresh in 
-  let e := fresh "e" in
-  evar (e: Prop); assert (H: reflect e X); subst e;
-  [eauto
-  | destruct H as [H|H]].
-
-Require Import Omega.
-
-Lemma reflect_iff P p : reflect P p -> p <-> P. destruct 1; split; auto; congruence. Qed.
-Hint Rewrite reflect_iff using solve [eauto] : bprop.
-Hint Rewrite <- reflect_iff using solve [eauto] : unprop.
-Ltac conv_to_prop := autorewrite with bprop in *.
-Ltac conv_from_prop := autorewrite with unprop in *.
-
-Goal forall x y z, x < y -> y < z -> x < z. intros. conv_to_prop. omega. Qed.
-
-Notation env a := (Expr.name -> option a).
-Variable (const_tys : env exp).
-Variable (conv : relation exp).
+Variable const_tys : env exp.
+(* Variable (conv : relation exp). *)
 
 (* Notation dget Gamma n := (nth (ids 0) Gamma n).[wk n.+1]. *)
 Fixpoint dget {T} `{Ids T} `{Subst T} (Gamma : seq T) (n : var) {struct n} : T :=
@@ -65,7 +48,7 @@ Inductive has_type (Gamma : seq exp) : exp ->  exp -> Prop :=
   T_bind : forall i, i < size Gamma -> [Gamma |+ Bind i :< dget Gamma i]
 | T_free : forall nm t, const_tys nm = Some t -> [Gamma |+ Free nm :< t]
 | T_sort : forall s, [Gamma |+ Sort s :< Sort s.+1]
-| T_cumu : forall i j, [Gamma |+ i :< Sort j] -> [Gamma |+ i :< Sort j.+1]
+(* | T_cumu : forall i j, [Gamma |+ i :< Sort j] -> [Gamma |+ i :< Sort j.+1] *)
 (* | T_set : [Gamma |+ Sort set :< Sort typ] *)
 | T_pi : forall A B u1 u2, [Gamma |+ A :< Sort u1] -> [(A :: Gamma) |+ B :< Sort u2] -> [Gamma |+ (A :>> B) :< Sort (imax u1 u2)]
 | T_lam : forall A B b, [(A :: Gamma) |+ b :< B] -> [Gamma |+ (Lam b) :< (A :>> B)]
@@ -83,6 +66,7 @@ Inductive has_type (Gamma : seq exp) : exp ->  exp -> Prop :=
               (* [(Sum A B :: Gamma) |+ P] -> *) 
                  [(    A   :: Gamma) |+ a              :< P.[Sum_inl (Bind 0) .: wk 1]] ->
                  [(      B :: Gamma) |+ b              :< P.[Sum_inr (Bind 0) .: wk 1]] ->
+                 [            Gamma  |+ ab             :< Sum A B] ->
                  (* [            Gamma  |+ Split P a b ab :< P.[ab/]] *)
                  [            Gamma  |+ Split a b ab   :< P.[ab/]]
                      
@@ -99,8 +83,13 @@ Inductive has_type (Gamma : seq exp) : exp ->  exp -> Prop :=
               [Gamma   |+ d :< Mu D] ->
               [Gamma   |+ mu D a d :< C.[d/]]
 
-| T_conv : forall A A', conv A A' -> forall a, [Gamma |+ a :< A] -> [Gamma |+ a :< A']
+(* | T_conv : forall A A', conv A A' -> forall a, [Gamma |+ a :< A] -> [Gamma |+ a :< A'] *)
+| T_wrap   : forall D d, [Gamma |+ d :< D_efunc D (Mu D)] -> [Gamma |+ d :< Mu D]
+| T_unwrap : forall D d, [Gamma |+ d :< Mu D] -> [Gamma |+ d :< D_efunc D (Mu D)]
+| T_subty : forall a A A', A ::< A' -> [Gamma |+ a :< A] -> [Gamma |+ a :< A']
 where "[ C |+ e :< t ]" := (has_type C e t).
+
+Hypothesis const_tys_vals : forall nm t e, const_tys nm = Some t /\ Reduction.const_vals nm = Some e -> [nil |+ e :< t].
 
 (* Fixpoint has_type_rec (Gamma : list exp) (e : exp) (T : exp) : Prop := *)
 (*   match e with *)
@@ -150,6 +139,23 @@ Lemma All_sub D : forall sigma C e, (All D C e).[sigma] = All D C.[up sigma] e.[
 Hint Resolve All_sub.
 Hint Rewrite All_sub.
 
+Hypothesis const_tys_closed : forall nm e, const_tys nm = Some e -> closed e.
+
+Hint Resolve const_tys_closed.
+Hint Resolve efunc_closed.
+Hint Resolve red_conv sred_cong1.
+
+Lemma conv_sub1 a b sigma : a <:::> b -> a.[sigma] <:::> b.[sigma]. 
+Proof. autorewrite with unconv; intros; destr_logic; eauto. Qed.
+Hint Resolve conv_sub1.
+
+Lemma subty_sub1 A A' sigma : A ::< A' -> A.[sigma] ::< A'.[sigma].
+Proof. induction 1; simpl in *; eauto using subtyp. 
+       assert (T1.[sigma] <:::> (Sort l1).[sigma]) by auto.
+       assert (T2.[sigma] <:::> (Sort l2).[sigma]) by auto.
+       eauto.
+Qed.
+Hint Resolve subty_sub1.
 
 Lemma ty_renaming xi Gamma Delta a A :
   [ Gamma |+ a :< A ] ->
@@ -158,7 +164,7 @@ Lemma ty_renaming xi Gamma Delta a A :
   [ Delta |+ a.[ren xi] :< A.[ren xi]].
 Proof. move=>Ha; move:xi Delta; induction Ha; simpl; intros; try solve[eauto].
        { rewrite H1; auto. }
-       { admit. }                (* needs closure properties for env *)
+       { rewrite closed_sub_id; try eapply const_tys_closed; eassumption || auto. }
        { asimpl. constructor; try solve[eauto].
          apply IHHa2; intros; simpl in *; auto.
          destruct v; simpl; solve[eauto].
@@ -184,7 +190,7 @@ Proof. move=>Ha; move:xi Delta; induction Ha; simpl; intros; try solve[eauto].
          replace P.[ab.[ren xi] .: ren xi] with P.[ren (upren xi)].[ab.[ren xi]/] by autosubst.
          apply T_split with (A := A.[ren xi]) (B := B.[ren xi]);
          match goal with [|- context[P.[?x].[?t .: ?r]]] => 
-                         replace P.[x].[t .: r] with P.[t .: r].[x] by autosubst end.
+                         replace P.[x].[t .: r] with P.[t .: r].[x] by autosubst | _ => apply IHHa3; solve[auto] end.
          { apply IHHa1; intros; destruct v; simpl in *; auto.
            - apply H; auto.
            - replace A.[wk 1].[ren (upren xi)] with A.[ren xi].[wk 1] by autosubst; reflexivity.
@@ -199,9 +205,12 @@ Proof. move=>Ha; move:xi Delta; induction Ha; simpl; intros; try solve[eauto].
          econstructor; auto.
          - apply IHHa1; auto; destruct v; simpl in *; intros; auto; apply H || rewrite <- H0; autosubst.           
          - asimpl; asimpl in IHHa2; exact IHHa2. }
-       { admit. }               (* needs conv sub props *)
-Admitted.
-(* CURRENT POINT *)
+       { apply T_wrap.
+         replace (D_efunc D (Mu D)) with (D_efunc D (Mu D)).[ren xi]; auto. }
+       { simpl in *. replace (D_efunc D (Mu D)).[ren xi] with (D_efunc D (Mu D)); auto.
+         symmetry. apply closed_sub_id; auto. }
+Qed.
+
 Lemma wk_i_up_jk : forall i j k, sub_eq (wk i >> upn j (wk k)) (upn (j - i) (wk k) >> wk i).
   intros i j.
   refine (sub_ind (fun j i ij => forall k, sub_eq (wk i >> upn j (wk k)) (upn ij (wk k) >> wk i)) _ _ _ j i); 
@@ -217,7 +226,7 @@ Hint Resolve wk_i_up_jk.
 (* Hint Rewrite sub_vars_tms using solve[eauto]. *)
 
 Lemma closed_upn : forall i j sigma, closed_sub j sigma -> closed_sub (i + j) (upn i sigma).
-  induction i; move=>j sigma; rewrite ?iterate_S; solve[eauto]. Qed.
+Proof. induction i; move=>j sigma; rewrite ?iterate_S; solve[eauto]. Qed.
 
 Hint Resolve closed_upn.
 
@@ -234,14 +243,15 @@ Lemma sub_var_cor : forall e Delta T, [Delta |+ e :< T] -> forall sigma Gamma, [
 Proof. induction 1; simpl; intros; auto;
   asimpl; rewrite <- ?subst_comp;
   try solve [eauto].
-  { admit. }               (* free vars need closure properties *)
+  { rewrite closed_sub_id; try eapply const_tys_closed; eassumption || eauto. }
   { replace B.[a.[sigma] .: sigma] with B.[up sigma].[a.[sigma]/]; solve[eauto]. }
   { econstructor; try replace B.[up sigma].[a.[sigma]/] with B.[a/].[sigma]; solve[auto]. }
   { replace B.[S_p1 s.[sigma] .: sigma] with B.[up sigma].[S_p1 s.[sigma]/]; solve[eauto]. }
   { replace P.[ab.[sigma] .: sigma] with P.[up sigma].[ab.[sigma]/] by autosubst. 
     econstructor. 
     { specialize (IHhas_type1 (up sigma)). asimpl in *. auto. }
-    { specialize (IHhas_type2 (up sigma)). asimpl in *. auto. } }
+    { specialize (IHhas_type2 (up sigma)). asimpl in *. auto. } 
+    { apply IHhas_type3; auto. } }
   { replace C.[d.[sigma] .: sigma] with C.[up sigma].[d.[sigma]/]; auto. econstructor; try solve[eauto].
     { eapply IHhas_type1. destruct x; intros.
       { asimpl. constructor; auto. }
@@ -252,8 +262,11 @@ Proof. induction 1; simpl; intros; auto;
       with (Mu D :>> (All D C.[up (wk 1)] (Bind 0) :>> C.[Bind 1 .: wk 2]).[up sigma]) 
         by (asimpl; rewrite All_sub; autosubst).
       eauto. } }
-  { admit. }               (* conv property *)
-Admitted.
+  { apply T_wrap.
+    replace (D_efunc D (Mu D)) with (D_efunc D (Mu D)).[sigma]; auto. }
+  { simpl in *; replace (D_efunc D (Mu D)).[sigma] with (D_efunc D (Mu D)); auto.
+    symmetry; apply closed_sub_id; auto. }
+Qed.
 
 Hint Resolve sub_var_cor.
 (* Notation "x .[ sigma ]" := (map (fun y => y.[sigma]) x). *)
@@ -262,35 +275,94 @@ Hint Rewrite <- subst_comp.
 Lemma sub_comp_cor Gamma Delta Sigma delta sigma : [Gamma |+ delta +| Delta] -> [Delta |+ sigma +| Sigma] -> [Gamma |+ sigma >> delta +| Sigma].
 Proof. intros; asimpl; autorewrite with core; solve[eauto]. Qed.
 
-Require Import Reduction.
+Lemma conv_pi_pi A B A' B' : (A :>> B) <:::> (A' :>> B') <-> (A <:::> A') /\ (B <:::> B').
+Proof. split; autorewrite with unconv; intros; destr_logic;eauto.
+       autorewrite with core in *; destr_logic; subst.
+       inverts H0. split; eexists; eauto. 
+Qed.
 
-Notation conv_con Gamma Delta := (size Gamma = size Delta /\ forall i, conv (dget Delta i) (dget Gamma i)). 
+Hint Rewrite conv_pi_pi.
 
-Hypothesis step_conv : forall e e', e ::> e' -> conv e e'.
-Hypothesis step_back_conv : forall e e', e ::> e' -> conv e' e.
-Hypothesis conv_refl : forall e, conv e e.
-Hypothesis conv_trans : forall e e' e'', conv e e' -> conv e' e'' -> conv e e''.
-Hypothesis conv_symm : forall e e', conv e e' -> conv e' e.
-Hypothesis conv_sub_congr1 : forall e e' sigma, conv e e' -> conv e.[sigma] e'.[sigma].
-Hypothesis conv_sub_congr : forall e e' sigma tau, sigma .>> tau -> conv e.[sigma] e'.[tau].
-Hint Resolve conv_refl conv_sub_congr1.
-Hint Resolve step_conv.
+Lemma T_conv Gamma e A B : A <:::> B -> [Gamma |+ e :< B] -> [Gamma |+ e :< A].
+Proof. intros; eapply T_subty; try (constructor; symmetry); eassumption. Qed.
 
-Lemma lam_pi Gamma A B b : [Gamma |+ Lam b :< A :>> B] -> [A :: Gamma |+ b :< B].
-Proof. remember (Lam b) as lb; remember (A :>> B) as ab.
-  induction 1; inversion Heqlb; inversion Heqab; subst; auto.
-(* Hint Extern 1 (conv (dget (?A :: ?Delta) ?i) (dget (?A' :: ?Gamma) ?i)) => destruct i; simpl. *)
-Theorem preservation Gamma Delta e e' T : conv_con Gamma Delta -> e ::> e' -> [Gamma |+ e :< T] -> [Delta |+ e' :< T].
-Proof. move=>Hgd He' He. move: e' He' Delta Hgd. 
-  induction He; simpl; intros; destruct Hgd as [Hl Hi]; inverts He'; try (try econstructor; solve[eauto]).
-  Local Hint Extern 1 (conv (dget (?A :: ?Delta) ?i) (dget (?A' :: ?Gamma) ?i)) => destruct i; simpl.
-  Hint Resolve step_back_conv.
-  { constructor. apply IHHe1; auto. apply IHHe2; auto; simpl; split; auto. }
-  { constructor. apply IHHe1; auto. apply IHHe2; auto. simpl; split; auto. }
-  { constructor. apply IHHe; auto. simpl; split; auto. }
-  { constructor. apply IHHe; auto. simpl; split; auto. }
-  { apply T_conv with (A := B.[a'/]); auto. apply T_app with (A := A); auto. }
-  { apply T_conv with (A := B.[a'/]); auto. 
-    assert (H: [Delta |+ Lam b :< (A :>> B)]) by auto.
-    - eapply sub_var_cor; try eassumption. inversion H; subst; try eassumption. 
-    - 
+Lemma closed_step e e' n : e ::> e' -> closed_at n e -> closed_at n e'.
+Proof. move=> He'; move: n; induction He'; simpl in *; intros;
+       autounfold in *; autorewrite with core in *; destr_logic;
+       try solve[repeat (apply andb_true_intro; split); auto].
+       - apply closed_lift with (i := 0); try eapply Reduction.const_vals_closed; eassumption || auto.
+       - apply cons_id_scoped; auto.
+       - htry; clear_funs. autorewrite with core in *; intuition.
+       - htry; clear_funs. autorewrite with core in *; intuition.
+       - htry; clear_funs. apply cons_id_scoped; auto.
+       - apply cons_id_scoped; auto.
+       - repeat split; auto.
+         apply rall_scoped; simpl; auto.
+         autounfold; autorewrite with core; intuition.
+         apply wk1_scoped; auto.
+Qed.
+
+Hint Resolve closed_step.
+
+(* TODO: Prove backward lemmas *)
+Lemma closed_wk1_back e n : closed_at n.+1 e.[wk 1] -> closed_at n e. Admitted.
+(* this one might be too strong - not sure *)
+Lemma closed_sub_back e a n : closed_at n e.[a/] -> closed_at n.+1 e /\ closed_at n a. Admitted.
+Hint Resolve closed_wk1_back closed_sub_back.
+Lemma closed_red e e' n : e :::> e' -> closed_at n e -> closed_at n e'.
+Proof. induction 1; intros; auto. eapply closed_step; eassumption. Qed.
+Hint Resolve closed_red.
+
+(* Lemma closed_conv e1 e2 n : e1 <:::> e2 -> closed_at n e1 -> closed_at n e2. *)
+(* Proof. induction 1; auto. eapply closed_step; eassumption.  *)
+       
+(* Lemma subty_closed n A B : A ::< B -> closed_at n A -> closed_at n B.  *)
+(* Proof. induction 1; intros; auto. *)
+(* Lemma lam_pi Gamma A B b : [Gamma |+ Lam b :< A :>> B] -> [A :: Gamma |+ b :< B]. *)
+(* Proof. remember (Lam b) as lb; remember (A :>> B) as ab. *)
+(*        (* assert (Lam b <:::> lb) by (subst; auto). *) *)
+(*        assert (Hc : A :>> B <:::> ab) by (subst; auto). *)
+(*        clear Heqab. move=>Hab;move:b Heqlb A B Hc. *)
+(*        induction Hab; intros; try solve by inversion. *)
+(*        { autorewrite with core in*; destr_logic. *)
+(*          inverts Heqlb. *)
+(*          replace b0 with b0.[ids] by autosubst. replace B0 with B0.[ids] by autosubst. *)
+(*          apply sub_var_cor with (Delta := A :: Gamma). *)
+(*          - eapply T_subty; eassumption || constructor; auto using symmetry. *)
+(*          - destruct x; intros; asimpl. *)
+(*            + eapply T_subty; eassumption || constructor; simpl; auto using symmetry. *)
+(*            + constructor; auto. } *)
+(*        { autorewrite with unconv in *; destr_logic. *)
+(*          apply red_Pi in H; apply red_Mu in H0; destr_logic; subst; congruence. } *)
+(*        { exfalso. clear IHHab Heqlb d b Hab d Gamma. *)
+(*          autorewrite with unconv in *; destr_logic. *)
+(*          apply red_Pi in H; destr_logic; subst. *)
+(*          destruct D; simpl in *;  *)
+(*          [apply red_Unit in H0|apply red_Mu in H0|apply red_Sum in H0|apply red_Sigma in H0]; *)
+(*          destr_logic; congruence. } *)
+(*        { subst. specialize (IHHab _  erefl). *)
+(*          assert (Haba' : A0 :>> B <:::> A). transitivity A'; auto using symmetry. *)
+(* by (eapply rst_trans; [|symmetry]; eassumption). *)
+(*          specialize (IHHab _ _ Haba'). *)
+(*          auto. } *)
+(* Qed. *)
+
+(* Lemma typed_closed Gamma e E : [Gamma |+ e :< E] -> closed_at (size Gamma) e. *)
+(* Proof. induction 1; simpl in *; repeat (apply andb_true_intro; split); auto 10. Qed. *)
+
+(* Print exp. *)
+
+(* (* Hint Extern 1 (conv (dget (?A :: ?Delta) ?i) (dget (?A' :: ?Gamma) ?i)) => destruct i; simpl. *) *)
+(* (* Theorem preservation Gamma Delta e e' T : conv_con Gamma Delta -> e ::> e' -> [Gamma |+ e :< T] -> [Delta |+ e' :< T]. *) *)
+(* (* Proof. move=>Hgd He' He. move: e' He' Delta Hgd.  *) *)
+(* (*   induction He; simpl; intros; destruct Hgd as [Hl Hi]; inverts He'; try (try econstructor; solve[eauto]). *) *)
+(* (*   Local Hint Extern 1 (conv (dget (?A :: ?Delta) ?i) (dget (?A' :: ?Gamma) ?i)) => destruct i; simpl. *) *)
+(* (*   Hint Resolve step_back_conv. *) *)
+(* (*   { constructor. apply IHHe1; auto. apply IHHe2; auto; simpl; split; auto. } *) *)
+(* (*   { constructor. apply IHHe1; auto. apply IHHe2; auto. simpl; split; auto. } *) *)
+(* (*   { constructor. apply IHHe; auto. simpl; split; auto. } *) *)
+(* (*   { constructor. apply IHHe; auto. simpl; split; auto. } *) *)
+(* (*   { apply T_conv with (A := B.[a'/]); auto. apply T_app with (A := A); auto. } *) *)
+(* (*   { apply T_conv with (A := B.[a'/]); auto.  *) *)
+(* (*     assert (H: [Delta |+ Lam b :< (A :>> B)]) by auto. *) *)
+(* (*     - eapply sub_var_cor; try eassumption. inversion H; subst; try eassumption.  *) *)
